expression progress progress

deps/coq-poulet4/lib/P4cub/TypeSoundness.v
@@ -5,10 +5,10 @@ Module P := P4cub.AST.P4cub.
 Module E := P.Expr.
 Module S := P.Stmt.
 Module V := Val.
+Import P.P4cubNotations.
 
 Import Typecheck.
 Import Step.
-Import P.P4cubNotations.
 Import V.ValueNotations.
 Import V.ValueTyping.
 Import F.FieldTactics.
@@ -21,6 +21,31 @@ Section BigStepTheorems.
     forall (x : name tags_t) (τ : E.t tags_t) (v : V.v tags_t),
       Γ x = Some τ -> ϵ x = Some v -> ∇ errs ⊢ v ∈ τ.
   (**[]*)
+
+  (** Epsilon is a subset of Gamma. *)
+  Definition envs_subset (Γ : gamma) (ϵ : epsilon) : Prop :=
+    forall (x : name tags_t) (τ : E.t tags_t),
+      Γ x = Some τ -> exists v, ϵ x = Some v.
+  (**[]*)
+
+  Definition envs_sound Γ ϵ errs : Prop :=
+    envs_type errs Γ ϵ /\ envs_subset Γ ϵ.
+  (**[]*)
+
+  Lemma envs_subset_type : forall Γ ϵ errs,
+      envs_subset Γ ϵ -> envs_type errs Γ ϵ.
+  Proof.
+    unfold envs_subset, envs_type.
+    intros Γ ϵ errs H x t v Ht Hv.
+    apply H in Ht as [v' Hv'].
+  Abort.
+
+  Lemma envs_type_subset : forall Γ ϵ errs,
+      envs_type errs Γ ϵ -> envs_subset Γ ϵ.
+  Proof.
+    unfold envs_subset, envs_type.
+    intros Γ ϵ errs H x t Ht.
+  Abort.
 
   Theorem expr_big_step_preservation :
     forall (errs : errors) (Γ : gamma) (e : E.e tags_t)
@@ -54,8 +79,7 @@ Section BigStepTheorems.
     - unfold eval_bit_binop in *; inv H; constructor.
     - inv H10.
     - inv H10.
-    - inv H8; constructor.
-      unfold BitArith.bit_concat; apply BitArith.return_bound_bound.
+    - unfold BitArith.bit_concat; apply BitArith.return_bound_bound.
     - apply IHHev1 in H10; auto; clear IHHev1.
       apply IHHev2 in H11; auto; clear IHHev2.
       destruct op; unfold eval_bit_binop in *;
@@ -102,4 +126,93 @@ Section BigStepTheorems.
       eapply Forall_nth_error in H11; eauto; simpl in *.
       inv H11; auto.
   Qed.
+
+  Theorem expr_big_step_progress :
+    forall (errs : errors) (Γ : gamma) (e : E.e tags_t)
+      (τ : E.t tags_t) (ϵ : epsilon),
+      envs_sound Γ ϵ errs ->
+      ⟦ errs, Γ ⟧ ⊢ e ∈ τ ->
+      exists v : V.v tags_t, ⟨ ϵ, e ⟩ ⇓ v.
+  Proof.
+    intros errs Γ τ e ϵ [Htyp Hsub] Ht.
+    unfold envs_subset, envs_type in *.
+    (* generalize dependent ϵ. *)
+    induction Ht using custom_check_ind;
+      (* intros ϵ Het; *)
+      try (eexists; constructor; assumption).
+    - apply Hsub in H. destruct H as [v H'].
+      exists v; constructor; auto.
+    - pose proof IHHt Htyp Hsub as [v IH]; clear IHHt.
+      pose proof expr_big_step_preservation _ _ _ _ _ _ Htyp IH Ht as Hpres.
+      inv Hpres. exists (V.VBool (negb b)); econstructor; eauto.
+    - pose proof IHHt Htyp Hsub as [v IH]; clear IHHt.
+      pose proof expr_big_step_preservation _ _ _ _ _ _ Htyp IH Ht as Hpres.
+      inv Hpres. exists (V.VBit w (BitArith.neg w n)); econstructor; eauto.
+    - pose proof IHHt Htyp Hsub as [v IH]; clear IHHt.
+      pose proof expr_big_step_preservation _ _ _ _ _ _ Htyp IH Ht as Hpres.
+      inv Hpres. exists (V.VInt w (IntArith.neg w z)); econstructor; eauto.
+    - pose proof IHHt1 Htyp Hsub as [v1 IH1]; clear IHHt1.
+      pose proof IHHt2 Htyp Hsub as [v2 IH2]; clear IHHt2.
+      pose proof expr_big_step_preservation _ _ _ _ _ _ Htyp IH1 Ht1 as HP1.
+      pose proof expr_big_step_preservation _ _ _ _ _ _ Htyp IH2 Ht2 as HP2.
+      inv H0; inv H2; inv H; inv HP1; inv HP2.
+      + remember (@eval_bit_binop tags_t op w n n0) as ebb eqn:eqnop.
+        inversion H1; subst op; simpl in *;
+          match goal with
+          | H: _ = Some ?v |- _ => exists v
+          end; econstructor; simpl in *; eauto.
+      + remember (@eval_int_binop tags_t op w z z0) as ebb eqn:eqnop.
+        inversion H1; subst op; simpl in *;
+          match goal with
+          | H: _ = Some ?v |- _ => exists v
+          end; econstructor; simpl in *; eauto.
+    - pose proof IHHt1 Htyp Hsub as [v1 IH1]; clear IHHt1.
+      pose proof IHHt2 Htyp Hsub as [v2 IH2]; clear IHHt2.
+      pose proof expr_big_step_preservation _ _ _ _ _ _ Htyp IH1 Ht1 as HP1.
+      pose proof expr_big_step_preservation _ _ _ _ _ _ Htyp IH2 Ht2 as HP2.
+      inv H0; inv H2; inv H; inv HP1; inv HP2.
+      + remember (@eval_bit_binop tags_t op w n n0) as ebb eqn:eqnop.
+        inversion H1; subst op; simpl in *;
+          match goal with
+          | H: _ = Some ?v |- _ => exists v
+          end; econstructor; simpl in *; eauto.
+      + remember (@eval_int_binop tags_t op w z z0) as ebb eqn:eqnop.
+        inversion H1; subst op; simpl in *;
+          match goal with
+          | H: _ = Some ?v |- _ => exists v
+          end; econstructor; simpl in *; eauto.
+    - pose proof IHHt1 Htyp Hsub as [v1 IH1]; clear IHHt1.
+      pose proof IHHt2 Htyp Hsub as [v2 IH2]; clear IHHt2.
+      pose proof expr_big_step_preservation _ _ _ _ _ _ Htyp IH1 Ht1 as HP1.
+      pose proof expr_big_step_preservation _ _ _ _ _ _ Htyp IH2 Ht2 as HP2.
+      inv HP1; inv HP2.
+      remember (eval_bool_binop op b b0) as ebb eqn:eqnop.
+      inversion H; subst op; simpl in *;
+        match goal with
+        | H: _ = Some ?b |- _ => exists (V.VBool b)
+        end; econstructor; simpl in *; eauto.
+    - pose proof IHHt1 Htyp Hsub as [v1 IH1]; clear IHHt1.
+      pose proof IHHt2 Htyp Hsub as [v2 IH2]; clear IHHt2.
+      exists (V.VBool (V.eqbv _ v1 v2)).
+      econstructor; eauto.
+    - pose proof IHHt1 Htyp Hsub as [v1 IH1]; clear IHHt1.
+      pose proof IHHt2 Htyp Hsub as [v2 IH2]; clear IHHt2.
+      exists (V.VBool (negb (V.eqbv _ v1 v2))).
+      econstructor; eauto.
+    - pose proof IHHt1 Htyp Hsub as [v1 IH1]; clear IHHt1.
+      pose proof IHHt2 Htyp Hsub as [v2 IH2]; clear IHHt2.
+      pose proof expr_big_step_preservation _ _ _ _ _ _ Htyp IH1 Ht1 as HP1.
+      pose proof expr_big_step_preservation _ _ _ _ _ _ Htyp IH2 Ht2 as HP2.
+      inv HP1; inv HP2.
+      exists (V.VBit (m + n) (BitArith.bit_concat m n n0 n1));
+        econstructor; eauto.
+    - pose proof IHHt Htyp Hsub as [v IH]; clear IHHt.
+      pose proof expr_big_step_preservation _ _ _ _ _ _ Htyp IH Ht as HP; inv HP.
+      eapply F.relfs_get_r in H2 as [v [Hget HR]]; eauto.
+      exists v. econstructor; eauto.
+    - pose proof IHHt Htyp Hsub as [v IH]; clear IHHt.
+      pose proof expr_big_step_preservation _ _ _ _ _ _ Htyp IH Ht as HP; inv HP.
+      eapply F.relfs_get_r in H2 as [v [Hget HR]]; eauto.
+      exists v. econstructor; eauto.
+  Abort.
 End BigStepTheorems.
